BinaryFv/RiscV/Step/Call.lean
@@ -65,6 +65,15 @@ theorem rX_bits_run_x10 (s : State) (data : BitVec 64)
     EStateM.get, EStateM.pure, EStateM.instMonad, EStateM.instMonadExceptOfOfBacktrackable,
     getThe, MonadState.get, MonadStateOf.get, stored]
 
+theorem rX_bits_run_x2 (s : State) (data : BitVec 64)
+    (stored : s.regs.get? x2 = some data) :
+    Runs (rX_bits (.Regidx 2#5)) s s data := by
+  have index : (Sail.BitVec.toNatInt (2#5 : BitVec 5)).toNat = 2 := rfl
+  unfold Runs
+  simp [rX_bits, rX, index, regval_from_reg, PreSail.readReg, EStateM.run, EStateM.bind,
+    EStateM.get, EStateM.pure, EStateM.instMonad, EStateM.instMonadExceptOfOfBacktrackable,
+    getThe, MonadState.get, MonadStateOf.get, stored]
+
 theorem wX_bits_run_x11 (s : State) (data : BitVec 64) :
     Runs (wX_bits (.Regidx 11#5) data) s { s with regs := s.regs.insert x11 data } () := by
   have hidx : (Sail.BitVec.toNatInt (11#5)).toNat = 11 := rfl
@@ -79,6 +88,15 @@ theorem rX_bits_run_x11 (s : State) (data : BitVec 64)
     (stored : s.regs.get? x11 = some data) :
     Runs (rX_bits (.Regidx 11#5)) s s data := by
   have index : (Sail.BitVec.toNatInt (11#5 : BitVec 5)).toNat = 11 := rfl
+  unfold Runs
+  simp [rX_bits, rX, index, regval_from_reg, PreSail.readReg, EStateM.run, EStateM.bind,
+    EStateM.get, EStateM.pure, EStateM.instMonad, EStateM.instMonadExceptOfOfBacktrackable,
+    getThe, MonadState.get, MonadStateOf.get, stored]
+
+theorem rX_bits_run_x18 (s : State) (data : BitVec 64)
+    (stored : s.regs.get? x18 = some data) :
+    Runs (rX_bits (.Regidx 18#5)) s s data := by
+  have index : (Sail.BitVec.toNatInt (18#5 : BitVec 5)).toNat = 18 := rfl
   unfold Runs
   simp [rX_bits, rX, index, regval_from_reg, PreSail.readReg, EStateM.run, EStateM.bind,
     EStateM.get, EStateM.pure, EStateM.instMonad, EStateM.instMonadExceptOfOfBacktrackable,
