BinaryFv/Zesu.lean
@@ -21,6 +21,7 @@ import BinaryFv.Zesu.MachineExecution.DecodeTactic
 import BinaryFv.Zesu.MachineExecution.BlobScheduleAndResultStores
 import BinaryFv.Zesu.MachineExecution.ParserBlocks
 import BinaryFv.Zesu.MachineExecution.AccessorBlocks
+import BinaryFv.Zesu.MachineExecution.Level2AllocatorProof
 import BinaryFv.Zesu.MemoryRepresentation.RawV4
 import BinaryFv.Zesu.MemoryRepresentation.Observers
 import BinaryFv.Zesu.MemoryRepresentation.Result
